feat (qs_partition) finish partition_pivot_correct

thys/examples/sorting/Sorting_Quicksort_Partition.thy
@@ -2,6 +2,17 @@ theory Sorting_Quicksort_Partition
 imports Sorting_Quicksort_Scheme
 begin
 
+(* TODO: move *)
+
+definition costmult :: "_ \<Rightarrow> ('b, _ ) acost \<Rightarrow> ('b, _ ) acost" (infixl "*m" 80)
+  where  "costmult s c \<equiv> acostC (\<lambda>x. s * the_acost c x)"
+
+lemma costmult_1_absorb[simp]: "(1::('b::comm_semiring_1)) *m c = c"
+  "(Suc 0) *m d = d"
+  by(simp_all add: costmult_def)
+
+
+
 hide_const pi
   
 (* TODO: Move. Found useful for ATPs *)
@@ -174,9 +185,6 @@ lemma move_median_to_first2_refine':
   apply(refine_rcg bindT_refine_conc_time_my_inres MIf_refine)
   by(auto intro: struct_preservingI)
 
-abbreviation costmult :: "enat \<Rightarrow> ('b, enat) acost \<Rightarrow> ('b, enat) acost" (infixl "*m" 80)
-  where  "costmult s c \<equiv> acostC (\<lambda>x. s * the_acost c x)"
-
 definition "move_median_to_first2_cost = 3 *m aa + cc + cost ''if'' 3"
 
 
@@ -191,6 +199,14 @@ lemma
   unfolding timerefineF_def timerefineA_def
   by auto
 
+
+thm timerefineA_update_apply_same_cost
+
+lemma timerefineA_update_apply_same_cost': 
+  "timerefineA (F(n := y)) (cost n (t::enat)) = t *m y"
+  by (auto simp: costmult_def timerefineA_def cost_def zero_acost_def timerefineA_upd_aux ) 
+
+print_classes
 
 lemma move_median_to_first2_correct: 
   "\<lbrakk> ri<ai; ai<bi; bi<ci; ci<length xs \<rbrakk> \<Longrightarrow> 
@@ -208,7 +224,7 @@ lemma move_median_to_first2_correct:
   subgoal apply(simp add: SPEC_timerefine_eq_arh)
     apply(rule SPEC_leq_SPEC_I) apply simp
     by(auto simp: move_median_to_first_cost_def move_median_to_first2_cost_def
-            timerefineA_update_apply_same_cost timerefineA_propagate add.assoc add.commute) 
+            timerefineA_update_apply_same_cost' timerefineA_propagate add.assoc add.commute) 
   by auto  
 
 
@@ -230,32 +246,124 @@ context weak_ordering begin
 subsection \<open>Hoare Partitioning Scheme\<close>  
 
 
-definition "ungrd_qsp_next_l_spec xs pi li hi \<equiv> 
+definition "ungrd_qsp_next_l_spec T xs pi li hi0 \<equiv> 
   doN {
-    ASSERT (pi<li \<and> pi<hi \<and> hi\<le>length xs);
-    ASSERT (\<exists>i\<in>{li..<hi}. xs!i \<^bold>\<ge> xs!pi); 
-    SPEC (\<lambda>li'. li\<le>li' \<and> li'<hi \<and> (\<forall>i\<in>{li..<li'}. xs!i\<^bold><xs!pi) \<and> xs!li'\<^bold>\<ge>xs!pi)
+    ASSERT (pi<li \<and> pi<hi0 \<and> hi0\<le>length xs);
+    ASSERT (\<exists>i\<in>{li..<hi0}. xs!i \<^bold>\<ge> xs!pi); 
+    SPEC (\<lambda>li'. li\<le>li' \<and> li'<hi0 \<and> (\<forall>i\<in>{li..<li'}. xs!i\<^bold><xs!pi) \<and> xs!li'\<^bold>\<ge>xs!pi) (\<lambda>li'. T li li')
   }"
 
-definition "ungrd_qsp_next_h_spec xs pi hi \<equiv> 
+definition "ungrd_qsp_next_h_spec T xs pi li0 hi \<equiv> 
   doN {
-    ASSERT (pi<length xs \<and> hi\<le>length xs \<and> (\<exists>i\<in>{pi<..<hi}. (xs!i) \<^bold>\<le> xs!pi)); 
-    SPEC (\<lambda>hi'. hi'<hi \<and> (\<forall>i\<in>{hi'<..<hi}. xs!i\<^bold>>xs!pi) \<and> xs!hi'\<^bold>\<le>xs!pi)
+    ASSERT (pi<li0 \<and> pi<length xs \<and> hi\<le>length xs \<and> (\<exists>i\<in>{li0..<hi}. (xs!i) \<^bold>\<le> xs!pi)); 
+    SPEC (\<lambda>hi'. li0\<le>hi' \<and> hi'<hi \<and> (\<forall>i\<in>{hi'<..<hi}. xs!i\<^bold>>xs!pi) \<and> xs!hi'\<^bold>\<le>xs!pi) (\<lambda>hi'. T hi hi')
   }"
+
+
+lemma "\<lbrakk>\<exists>i\<in>{li0..<hi}. xs ! i \<^bold>\<le> xs!pi; (\<forall>i\<in>{xa'<..<hi}. xs ! pi \<^bold>< xs! i) \<rbrakk> \<Longrightarrow> li0 \<le> xa'" 
+    by (meson atLeastLessThan_iff greaterThanLessThan_iff leI less_le_trans wo_leD)
+
   
   
-definition qsp_next_l :: "'a list \<Rightarrow> nat \<Rightarrow> nat \<Rightarrow> nat \<Rightarrow> nat nres" where            
+definition qsp_next_l :: "'a list \<Rightarrow> nat \<Rightarrow> nat \<Rightarrow> nat \<Rightarrow> (nat, ecost) nrest" where            
   "qsp_next_l xs pi li hi \<equiv> doN {
     monadic_WHILEIT (\<lambda>li'. (\<exists>i\<in>{li'..<hi}. xs!i\<^bold>\<ge>xs!pi) \<and> li\<le>li' \<and> (\<forall>i\<in>{li..<li'}. xs!i\<^bold><xs!pi)) 
-      (\<lambda>li. doN {ASSERT (li\<noteq>pi); mop_cmp_idxs xs li pi}) (\<lambda>li. RETURN (li + 1)) li
+      (\<lambda>li. doN {ASSERT (li\<noteq>pi); mop_cmp_idxs (cost ''cmp_idxs'' 1) xs li pi}) (\<lambda>li. SPECc2 ''add'' (+) li 1) li
   }"  
 
-  
-lemma qsp_next_l_refine: "(qsp_next_l,PR_CONST ungrd_qsp_next_l_spec)\<in>Id\<rightarrow>Id\<rightarrow>Id\<rightarrow>Id\<rightarrow>\<langle>Id\<rangle>nres_rel"
-  unfolding qsp_next_l_def ungrd_qsp_next_l_spec_def PR_CONST_def
-  apply (intro fun_relI; clarsimp)
+
+lemma if_rule: "(c \<Longrightarrow> x \<le> a) \<Longrightarrow> (~c \<Longrightarrow> x \<le> b) \<Longrightarrow> x \<le> (if c then a else b)"
+  by auto
+
+definition uqnl_body 
+  where "uqnl_body \<equiv> (cost ''if'' (1) + cost ''call'' 1
+                                                            + cost ''cmp_idxs'' 1)"
+definition "ungrd_qsp_next_l_cost li li' = (enat(li'-li+1)) *m uqnl_body + cost ''add'' (enat(li'-li))"
+
+
+lemma costmult_add_distrib:
+  fixes a :: "'b::semiring"
+  shows "a *m (c + d) = a *m c + a *m d"
+  apply(cases c; cases d) by (auto simp: costmult_def plus_acost_alt ring_distribs)
+
+lemma costmult_minus_distrib2:
+  fixes a :: nat
+  shows "a *m c - a *m d = a *m (c - d)"
+  apply(cases c; cases d) by (auto simp: costmult_def plus_acost_alt diff_mult_distrib2)
+
+lemma costmult_minus_distrib:
+  fixes a :: nat
+  shows "a *m c - b *m c = (a-b) *m c"
+  apply(cases c) by (auto simp: costmult_def plus_acost_alt diff_mult_distrib)
+
+lemma costmult_cost:
+  fixes x :: "'b::comm_semiring_1"
+  shows "x *m (cost n y) = cost n (x*y)"
+  by(auto simp: costmult_def cost_def zero_acost_def)
+
+(*
+lemma fixes a :: enat
+  shows "b\<le>a \<Longrightarrow> a *m x - b *m x = (a-b) *m x"
+  apply(auto simp: costmult_def minus_acost_alt intro!: ext)
+  done *)
+
+lemma qsp_next_l_refine: "(qsp_next_l,PR_CONST (ungrd_qsp_next_l_spec ungrd_qsp_next_l_cost))\<in>Id\<rightarrow>Id\<rightarrow>Id\<rightarrow>Id\<rightarrow>\<langle>Id\<rangle>nrest_rel"
+  unfolding qsp_next_l_def ungrd_qsp_next_l_spec_def ungrd_qsp_next_l_cost_def PR_CONST_def
+  apply (intro fun_relI nrest_relI; clarsimp)
+  apply(rule le_acost_ASSERTI)+
+  unfolding SPEC_def mop_cmp_idxs_def SPECc2_def
   subgoal for xs p li hi
-    apply (refine_vcg monadic_WHILEIT_rule[where R="measure (\<lambda>li. hi - li)"])
+    apply(subst monadic_WHILEIET_def[symmetric, where E="\<lambda>li'. (hi-li') *m (uqnl_body + cost ''add'' 1)"])
+    apply(rule gwp_specifies_I) 
+    apply (refine_vcg \<open>-\<close>  rules: gwp_monadic_WHILEIET if_rule)
+    subgoal 
+      unfolding wfR2_def apply (auto simp: uqnl_body_def costmult_add_distrib costmult_cost the_acost_propagate zero_acost_def)
+      by(auto simp: cost_def zero_acost_def) 
+    subgoal for li'
+      apply(rule loop_body_conditionI)
+      subgoal apply(simp add: uqnl_body_def costmult_add_distrib costmult_cost lift_acost_propagate lift_acost_cost)
+        apply sc_solve 
+        by auto
+      subgoal apply(simp add: uqnl_body_def costmult_add_distrib costmult_cost lift_acost_propagate lift_acost_cost)
+        apply sc_solve 
+        apply safe
+        subgoal apply auto  
+          by (metis Suc_eq_plus1 Suc_n_not_le_n add.commute le_diff_iff' le_trans lift_ord lt_by_le_def lt_by_linorder not_less_eq_eq one_enat_def plus_enat_simps(1))  
+        subgoal apply auto  
+          by (simp add: one_enat_def)  
+        subgoal apply auto  
+          by (simp add: one_enat_def)  
+        subgoal apply (auto simp add: one_enat_def)
+          done
+        done
+      subgoal 
+        by (metis One_nat_def add.commute atLeastLessThan_iff less_Suc_eq less_Suc_eq_le linorder_not_le plus_1_eq_Suc wo_leD)
+      done
+    subgoal for li'
+      apply(rule loop_exit_conditionI)
+      apply(rule if_rule2)
+      subgoal apply(subst costmult_minus_distrib) apply simp
+        unfolding uqnl_body_def apply(simp add: costmult_add_distrib costmult_cost lift_acost_propagate lift_acost_cost)
+        apply sc_solve
+        apply safe
+        subgoal apply auto
+          by (metis Suc_diff_le add.commute eq_iff one_enat_def plus_1_eq_Suc plus_enat_simps(1))
+        subgoal apply auto
+          by (metis Suc_diff_le eq_iff one_enat_def plus_1_eq_Suc plus_enat_simps(1))
+        subgoal apply auto
+          by (metis Suc_diff_le add.commute eq_iff one_enat_def plus_1_eq_Suc plus_enat_simps(1))
+        subgoal by auto
+        done
+      subgoal by (auto simp: unfold_le_to_lt)
+      done
+    subgoal apply auto done
+    subgoal apply auto done
+    subgoal apply auto done
+    done
+  done
+
+(*
+    oops
     apply simp_all
     subgoal by auto
     apply safe
@@ -266,21 +374,97 @@ lemma qsp_next_l_refine: "(qsp_next_l,PR_CONST ungrd_qsp_next_l_spec)\<in>Id\<ri
     subgoal by (auto simp: unfold_le_to_lt)
     done  
   done
+*)
 
-
-definition qsp_next_h :: "'a list \<Rightarrow> nat \<Rightarrow> nat \<Rightarrow> nat nres" where
-  "qsp_next_h xs pi hi \<equiv> doN {
+definition qsp_next_h :: "'a list \<Rightarrow> nat  \<Rightarrow> nat \<Rightarrow> nat \<Rightarrow> (nat, ecost) nrest" where
+  "qsp_next_h xs pi li0 hi \<equiv> doN {
     ASSERT (hi>0);
-    let hi = hi - 1;
+    hi \<leftarrow> SPECc2 ''sub'' (-) hi 1;
     ASSERT (hi<length xs);
     monadic_WHILEIT (\<lambda>hi'. hi'\<le>hi \<and> (\<exists>i\<le>hi'. xs!i\<^bold>\<le>xs!pi) \<and> (\<forall>i\<in>{hi'<..hi}. xs!i\<^bold>>xs!pi))
-      (\<lambda>hi. doN {ASSERT(pi\<noteq>hi); mop_cmp_idxs xs pi hi}) (\<lambda>hi. doN { ASSERT(hi>0); RETURN (hi - 1)}) hi
+      (\<lambda>hi. doN {ASSERT(pi\<noteq>hi); mop_cmp_idxs (cost ''cmp_idxs'' 1) xs pi hi})
+      (\<lambda>hi. doN { ASSERT(hi>0); SPECc2 ''sub'' (-) hi 1}) hi
   }"  
 
+definition uqnr_body 
+  where "uqnr_body \<equiv> (cost ''if'' (1) + cost ''call'' 1
+                                                           + cost ''sub'' 1 + cost ''cmp_idxs'' 1)"
+definition "ungrd_qsp_next_r_cost hi hi' =  (enat(hi-hi')) *m uqnr_body"
   
-lemma qsp_next_h_refine: "(qsp_next_h,PR_CONST (ungrd_qsp_next_h_spec)) \<in> Id \<rightarrow> Id \<rightarrow> Id \<rightarrow> \<langle>Id\<rangle>nres_rel"
-  unfolding qsp_next_h_def ungrd_qsp_next_h_spec_def PR_CONST_def
-  apply (refine_vcg monadic_WHILEIT_rule[where R="measure id"] split_ifI)
+lemma tt: "hi>0 \<Longrightarrow> {hi'<..hi - Suc 0} = {hi'<..<hi}" by auto
+
+lemma qsp_next_h_refine: "(qsp_next_h,PR_CONST (ungrd_qsp_next_h_spec ungrd_qsp_next_r_cost)) \<in> Id  \<rightarrow> Id \<rightarrow> Id \<rightarrow> Id \<rightarrow> \<langle>Id\<rangle>nrest_rel"
+  unfolding qsp_next_h_def ungrd_qsp_next_h_spec_def ungrd_qsp_next_r_cost_def PR_CONST_def 
+  apply (intro fun_relI nrest_relI; clarsimp)
+  apply(rule le_acost_ASSERTI)+
+  unfolding SPEC_def SPECc2_def mop_cmp_idxs_def
+  subgoal for xs pi li0 hi
+    apply(subst monadic_WHILEIET_def[symmetric, where E="\<lambda>hi'. (hi'-li0) *m uqnr_body"])
+    apply(rule gwp_specifies_I) 
+    apply (refine_vcg \<open>-\<close> rules: gwp_monadic_WHILEIET if_rule split_ifI)
+    subgoal
+      unfolding wfR2_def apply (auto simp: uqnr_body_def costmult_add_distrib costmult_cost the_acost_propagate zero_acost_def)
+      by(auto simp: cost_def zero_acost_def) 
+    subgoal 
+      apply(rule loop_body_conditionI)
+      subgoal 
+        apply(simp add: uqnr_body_def costmult_add_distrib costmult_cost lift_acost_propagate lift_acost_cost)
+        apply sc_solve 
+        apply safe by auto
+      subgoal apply(simp add: uqnr_body_def costmult_add_distrib costmult_cost lift_acost_propagate lift_acost_cost)
+        apply sc_solve 
+        apply safe
+        subgoal apply auto
+          by (metis Suc_diff_Suc eq_iff greaterThanAtMost_iff less_le_trans nat_le_Suc_less_imp nat_neq_iff one_enat_def plus_1_eq_Suc plus_enat_simps(1) wo_leD) 
+        subgoal apply auto 
+          by (metis Suc_diff_Suc add.commute diff_is_0_eq eq_iff greaterThanAtMost_iff le_less_trans nat_le_Suc_less_imp not_gr_zero one_enat_def plus_1_eq_Suc plus_enat_simps(1) wo_leD zero_less_diff)
+        subgoal apply auto 
+          by (metis Suc_diff_Suc diff_is_0_eq eq_iff greaterThanAtMost_iff le_less_trans nat_le_Suc_less_imp not_gr_zero one_enat_def plus_1_eq_Suc plus_enat_simps(1) wo_leD zero_less_diff)
+        subgoal apply auto 
+          by (metis Suc_diff_Suc add.commute diff_is_0_eq eq_iff greaterThanAtMost_iff le_less_trans nat_le_Suc_less_imp not_gr_zero one_enat_def plus_1_eq_Suc plus_enat_simps(1) wo_leD zero_less_diff)
+        done
+      subgoal apply auto 
+        subgoal by (metis One_nat_def le_step_down_nat wo_leD)
+        subgoal by (metis Suc_lessI Suc_pred greaterThanAtMost_iff)  
+        done
+      done
+    subgoal apply auto  
+      by (metis gr0I leD wo_leD)  
+    subgoal for hi'
+      apply(rule loop_exit_conditionI)
+      apply(rule if_rule2)
+      subgoal  apply(subst costmult_minus_distrib) apply simp
+        unfolding uqnr_body_def apply(simp add:  costmult_add_distrib costmult_cost lift_acost_propagate lift_acost_cost)
+        apply sc_solve
+        apply(simp add: zero_enat_def one_enat_def) (*
+        apply safe
+        subgoal by linarith
+        subgoal by linarith 
+        subgoal
+          using \<open>\<And>ia i. \<lbrakk>hi - Suc 0 < length xs; pi \<noteq> hi'; pi < length xs; \<not> xs ! pi \<^bold>< xs ! hi'; cost ''if'' (hi' - pi) + (cost ''call'' (hi' - pi) + (cost ''sub'' (hi' - pi) + cost ''cmp_idxs'' (hi' - pi))) \<le> cost ''if'' (hi - Suc pi) + (cost ''call'' (hi - Suc pi) + (cost ''sub'' (hi - Suc pi) + cost ''cmp_idxs'' (hi - Suc pi))); hi \<le> length xs; i \<in> {pi<..<hi}; xs ! i \<^bold>\<le> xs ! pi; hi' \<le> hi - Suc 0; hi' < hi; \<forall>i\<in>{hi'<..hi - Suc 0}. xs ! pi \<^bold>< xs ! i; \<forall>i\<in>{hi'<..<hi}. xs ! pi \<^bold>< xs ! i; xs ! hi' \<^bold>\<le> xs ! pi; ia \<le> hi'; xs ! ia \<^bold>\<le> xs ! pi\<rbrakk> \<Longrightarrow> Suc (hi - Suc (pi + (hi' - pi))) \<le> hi - hi'\<close> by blast
+        *) done
+      subgoal
+        apply (intro conjI) 
+        subgoal unfolding tt  by (meson atLeastLessThan_iff greaterThanLessThan_iff leI less_le_trans wo_leD)  
+        subgoal using nat_le_Suc_less by blast
+        subgoal by (simp add: nat_le_Suc_less_imp)
+        subgoal using wo_leI by blast
+        done
+      done
+    subgoal by auto 
+    subgoal by (meson atLeastLessThan_iff dual_order.strict_trans1 greaterThanAtMost_iff nat_le_Suc_less_imp wo_leD) 
+    subgoal apply auto
+      using nat_le_Suc_less_imp by blast  
+    subgoal          
+      using nz_le_conv_less by blast  
+    subgoal  
+      by auto  
+    done
+  done
+
+
+  (*
+
   apply (all \<open>(determ \<open>elim conjE exE\<close>)?\<close>)
   apply simp_all
   subgoal by force
@@ -291,18 +475,19 @@ lemma qsp_next_h_refine: "(qsp_next_h,PR_CONST (ungrd_qsp_next_h_spec)) \<in> Id
   subgoal by (metis Suc_pred greaterThanAtMost_iff linorder_neqE_nat not_less_eq)
   subgoal by (meson greaterThanAtMost_iff greaterThanLessThan_iff nat_le_Suc_less_imp)
   subgoal using wo_leI by blast
-  done  
+  done  *)
 
+definition "guard x = x"
 definition "qs_partition li\<^sub>0 hi\<^sub>0 pi xs\<^sub>0 \<equiv> doN {
   ASSERT (pi < li\<^sub>0 \<and> li\<^sub>0<hi\<^sub>0 \<and> hi\<^sub>0\<le>length xs\<^sub>0);
   
   \<comment> \<open>Initialize\<close>
-  li \<leftarrow> ungrd_qsp_next_l_spec xs\<^sub>0 pi li\<^sub>0 hi\<^sub>0;
-  hi \<leftarrow> ungrd_qsp_next_h_spec xs\<^sub>0 pi hi\<^sub>0;
+  li \<leftarrow> ungrd_qsp_next_l_spec ungrd_qsp_next_l_cost xs\<^sub>0 pi li\<^sub>0 hi\<^sub>0;
+  hi \<leftarrow> ungrd_qsp_next_h_spec ungrd_qsp_next_r_cost xs\<^sub>0 pi li\<^sub>0 hi\<^sub>0;
   
   ASSERT (li\<^sub>0\<le>hi);
   
-  (xs,li,hi) \<leftarrow> WHILEIT 
+  (xs,li,hi) \<leftarrow> monadic_WHILEIT 
     (\<lambda>(xs,li,hi). 
         li\<^sub>0\<le>li \<and> hi<hi\<^sub>0
       \<and> li<hi\<^sub>0 \<and> hi\<ge>li\<^sub>0  
@@ -313,13 +498,13 @@ definition "qs_partition li\<^sub>0 hi\<^sub>0 pi xs\<^sub>0 \<equiv> doN {
       \<and> (\<forall>i\<in>{hi<..<hi\<^sub>0}. xs!i \<^bold>\<ge> xs\<^sub>0!pi)
       \<and> xs!hi \<^bold>\<le> xs\<^sub>0!pi  
     )
-    (\<lambda>(xs,li,hi). li<hi) 
+    (\<lambda>(xs,li,hi). SPECc2 ''lt'' (<) li hi) 
     (\<lambda>(xs,li,hi). doN {
       ASSERT(li<hi \<and> li<length xs \<and> hi<length xs \<and> li\<noteq>hi);
-      xs \<leftarrow> mop_list_swap xs li hi;
-      let li = li + 1;
-      li \<leftarrow> ungrd_qsp_next_l_spec xs pi li hi\<^sub>0;
-      hi \<leftarrow> ungrd_qsp_next_h_spec xs pi hi;
+      xs \<leftarrow> mop_list_swapN xs li hi;
+      li \<leftarrow> SPECc2 ''add'' (+) li 1;
+      li \<leftarrow> ungrd_qsp_next_l_spec ungrd_qsp_next_l_cost xs pi li hi\<^sub>0;
+      hi \<leftarrow> ungrd_qsp_next_h_spec ungrd_qsp_next_r_cost xs pi li\<^sub>0 hi;
       RETURN (xs,li,hi)
     }) 
     (xs\<^sub>0,li,hi);
@@ -327,11 +512,186 @@ definition "qs_partition li\<^sub>0 hi\<^sub>0 pi xs\<^sub>0 \<equiv> doN {
   RETURN (xs,li)
 }"  
 
+
+definition uqnlr_body 
+  where "uqnlr_body \<equiv> (cost ''list_swap'' 1 + cost ''add'' 1 + cost ''if'' 3 + cost ''call'' 3
+                         + cost ''sub'' 1 + cost ''cmp_idxs'' 2)"
+
+abbreviation "qs_body_cost \<equiv> (cost ''add'' (1::enat) + cost ''sub'' 1
+      + cost ''list_swap'' 1 + cost ''if'' 3 + cost ''call'' 3 + cost ''lt'' 1 + cost ''cmp_idxs'' 2)"
+definition "qs_partition_cost xs\<^sub>0 li hi = (enat (hi-li)) *m qs_body_cost"
+
+lemma qs_partition_correct_aux1:
+  fixes hi'' :: nat
+  assumes "hi''\<ge>li''" and "hi'\<ge>li'"
+  shows "hi'' - li'' + hi' + li'' - (hi'' + li') \<le> hi' - li'"
+proof -
+  have "hi'' - li'' + hi' + li'' - (hi'' + li')
+        = hi' + (hi'' - li'' +  li'') - (hi'' + li')"
+    by auto
+  also have  "\<dots> = hi' + hi'' - (hi'' + li')"
+    using assms(1) by simp
+  also have "\<dots> = hi' - li'"
+    using assms(2) by simp
+  finally show ?thesis by simp    
+qed
+
+lemma pff:
+  assumes "hi''<hi'" "li'<li''"
+  shows "( (hi''::int) - li'') * 2 + hi' + li'' - (hi'' + li') \<le> (hi' - li') * 2"
+  using assms(1) assms(2) by auto
+
+lemma
+  assumes   "li'<li''"  "hi''<hi'" (* "li<li'" "hi'<hi" "li<hi" "li'<hi'" *)
+  shows "(1::int) + (hi'' - li'' + (hi'' - li + (hi + hi'))) - (hi'' + li') \<le> hi' + hi' + hi - (li' + li + li')"
+  using assms by simp
+
+lemma woaleack:
+  assumes A: "li'<li''" "li''<hi" and B: "hi''<hi'" "li<hi''" and C: "hi''<hi'" "li'<li''" "li'<hi'"
+  shows "(hi''::nat) - li'' + (hi'' - li) + (hi - li'') + (hi' - hi'') + (li'' - li') + 1 \<le> 0 + (hi' - li') + (hi' - li) + (hi - li')"
+proof -
+  have *: "((hi - li'') + (li'' - li')) = hi - li'"
+    using A by auto
+  have **: "(hi' - hi'') + (hi'' - li) = hi' - li"
+    using B by auto
+  have ***: "((hi'' - li'') + 1) \<le> (hi' - li')"
+    using C by auto    
+  have "hi'' - li'' + (hi'' - li) + (hi - li'') + (hi' - hi'') + (li'' - li') + 1 
+      = ((hi - li'') + (li'' - li')) + ((hi' - hi'') + (hi'' - li)) + ((hi'' - li'') + 1)"
+    by simp
+  also have "\<dots> = ((hi - li') + (hi' - li)) + ((hi'' - li'') + 1)" using * ** by simp
+  also have "\<dots> \<le> ((hi - li') + (hi' - li)) + (hi' - li')"
+    apply(rule add_left_mono) apply(subst ***) by simp 
+  also have "\<dots> = 0 + (hi' - li') + (hi' - li) + (hi - li')" by simp
+  finally show ?thesis .
+qed
+ 
 lemma qs_partition_correct:
+  fixes xs\<^sub>0 :: "'a list"
+  shows 
   "\<lbrakk> pi<li; li<hi; hi\<le>length xs\<^sub>0; \<exists>i\<in>{li..<hi}. xs\<^sub>0!pi\<^bold>\<le>xs\<^sub>0!i; \<exists>i\<in>{li..<hi}. xs\<^sub>0!i\<^bold>\<le>xs\<^sub>0!pi \<rbrakk> \<Longrightarrow> qs_partition li hi pi xs\<^sub>0 
-  \<le> SPEC (\<lambda>(xs,i). slice_eq_mset li hi xs xs\<^sub>0 \<and> li\<le>i \<and> i<hi \<and> (\<forall>i\<in>{li..<i}. xs!i\<^bold>\<le>xs\<^sub>0!pi) \<and> (\<forall>i\<in>{i..<hi}. xs!i\<^bold>\<ge>xs\<^sub>0!pi) )"  
+  \<le> SPEC (\<lambda>(xs,i). slice_eq_mset li hi xs xs\<^sub>0 \<and> li\<le>i \<and> i<hi \<and> (\<forall>i\<in>{li..<i}. xs!i\<^bold>\<le>xs\<^sub>0!pi) \<and> (\<forall>i\<in>{i..<hi}. xs!i\<^bold>\<ge>xs\<^sub>0!pi) ) (\<lambda>_. qs_partition_cost xs\<^sub>0 li hi )"  
   unfolding qs_partition_def ungrd_qsp_next_l_spec_def ungrd_qsp_next_h_spec_def
-  apply (refine_vcg WHILEIT_rule[where R="measure (\<lambda>(_,_,hi). hi)"])  
+  unfolding SPEC_REST_emb'_conv  SPECc2_def mop_list_swap_def
+  
+  apply(rule gwp_specifies_I)
+
+  apply(subst monadic_WHILEIET_def[symmetric, where E="\<lambda>(xs::'a list,li'::nat,hi'::nat).
+             (hi-li') *m (uqnl_body+ cost ''add'' 1) + (hi'-li) *m uqnr_body + (hi'-li') *m (cost ''list_swap'' 1 + cost ''call'' 1 + cost ''lt'' 1 + cost ''if'' 1) "])
+  apply (refine_vcg \<open>-\<close> rules: gwp_RETURNT_I gwp_monadic_WHILEIET if_rule split_ifI)  
+ 
+  subgoal unfolding wfR2_def 
+    apply safe
+    apply (auto simp add: uqnl_body_def uqnr_body_def costmult_add_distrib costmult_cost   the_acost_propagate)
+    apply (simp_all add: cost_def zero_acost_def)
+    done  
+  subgoal  for _ _ _ xs li' hi' li'' hi'' 
+    apply(rule loop_body_conditionI)
+    subgoal 
+      unfolding ungrd_qsp_next_l_cost_def ungrd_qsp_next_r_cost_def 
+            uqnlr_body_def uqnl_body_def uqnr_body_def
+      apply(simp add: costmult_add_distrib costmult_cost lift_acost_cost lift_acost_propagate)
+      apply sc_solve  by auto   
+    subgoal apply simp
+      unfolding ungrd_qsp_next_l_cost_def ungrd_qsp_next_r_cost_def 
+            uqnlr_body_def uqnl_body_def uqnr_body_def
+      apply(simp add: costmult_add_distrib costmult_cost lift_acost_cost lift_acost_propagate)
+      apply sc_solve_debug
+      apply safe
+      subgoal (* ''list_swap'' *) unfolding sc_solve_debug_def by (simp add: zero_enat_def one_enat_def)
+      subgoal (* ''if'' *) unfolding sc_solve_debug_def
+        apply(simp only: zero_enat_def one_enat_def plus_enat_simps lift_ord) done
+      subgoal unfolding sc_solve_debug_def by (simp add: one_enat_def)
+      subgoal unfolding sc_solve_debug_def by (simp add: one_enat_def)
+      subgoal (* ''add'' *) unfolding sc_solve_debug_def 
+        by(simp only: zero_enat_def one_enat_def plus_enat_simps lift_ord) 
+      subgoal (* ''cmp_idxs'' *) unfolding sc_solve_debug_def 
+        by(simp only: zero_enat_def one_enat_def plus_enat_simps lift_ord) 
+      subgoal (* ''sub'' *) unfolding sc_solve_debug_def 
+        by (simp only: zero_enat_def one_enat_def plus_enat_simps lift_ord) 
+      done
+    subgoal 
+      apply safe
+      subgoal by linarith
+      subgoal by linarith
+      subgoal by (metis atLeastLessThan_iff slice_eq_mset_swap(2) swap_length)
+      subgoal by (metis leD swap_indep)
+      subgoal apply(simp only: unfold_lt_to_le) apply clarsimp
+        apply (smt Suc_leI atLeastLessThan_iff le_def less_le_trans less_Suc_eq swap_indep swap_length swap_nth1)
+        done
+      subgoal by (metis (full_types) linorder_not_le swap_indep)
+      subgoal
+          (* this proof is even more crazy *)
+        apply(use [[put_named_ss HOL_ss]] in \<open>clarsimp\<close>) 
+        apply(use [[put_named_ss Main_ss]] in \<open>simp_all add: slice_eq_mset_eq_length unfold_lt_to_le\<close>)   
+        apply clarsimp 
+        by (metis greaterThanLessThan_iff less_le_trans linorder_neqE_nat swap_indep swap_nth2) 
+      subgoal by (metis (full_types) linorder_not_le swap_indep)
+      done
+    done
+  subgoal apply safe
+    subgoal by linarith
+    subgoal by linarith
+    subgoal by (metis atLeastLessThan_iff linwo swap_indep swap_nth1 weak_ordering.unfold_lt_to_le)
+    done
+  subgoal by (metis atLeastLessThan_iff discrete less_not_refl linwo swap_indep swap_nth2 weak_ordering.wo_less_le_trans)
+  subgoal apply safe
+    subgoal by linarith
+    subgoal by (simp add: slice_eq_mset_eq_length) 
+    done
+  subgoal by safe
+  subgoal apply safe
+    subgoal by (metis (full_types) less_le_trans slice_eq_mset_eq_length)
+    subgoal by (metis (full_types) less_le_trans slice_eq_mset_eq_length)
+    done
+  subgoal
+    apply(rule loop_exit_conditionI)
+    apply(rule gwp_RETURNT_I)
+    unfolding emb'_def
+    apply(rule if_rule2)
+    subgoal 
+      apply(subst lift_acost_diff_to_the_right) subgoal 
+        by(simp add: cost_zero costmult_add_distrib costmult_cost lift_acost_cost lift_acost_propagate)
+      unfolding ungrd_qsp_next_r_cost_def ungrd_qsp_next_l_cost_def
+      unfolding    uqnlr_body_def uqnl_body_def uqnr_body_def
+      apply simp
+      unfolding qs_partition_cost_def
+      apply(simp add: cost_zero costmult_add_distrib costmult_cost lift_acost_cost lift_acost_propagate)
+      apply sc_solve_debug
+      apply safe
+      subgoal unfolding sc_solve_debug_def by (simp add: one_enat_def numeral_eq_enat)
+      subgoal unfolding sc_solve_debug_def by (simp add: one_enat_def numeral_eq_enat)
+      subgoal (* ''cmp_idxs'' *) unfolding sc_solve_debug_def by (simp add: one_enat_def numeral_eq_enat)
+      subgoal unfolding sc_solve_debug_def by (simp add: one_enat_def numeral_eq_enat)
+      subgoal unfolding sc_solve_debug_def by (simp add: one_enat_def numeral_eq_enat)
+      subgoal unfolding sc_solve_debug_def by (simp add: one_enat_def numeral_eq_enat)
+      subgoal unfolding sc_solve_debug_def by (simp add: one_enat_def numeral_eq_enat)
+      done
+    subgoal 
+      apply safe
+      by (metis atLeastLessThan_iff greaterThanLessThan_iff le_eq_less_or_eq strict_itrans)
+    done
+  subgoal apply simp
+    apply safe
+    subgoal using unfold_lt_to_le by blast
+    subgoal using unfold_lt_to_le by blast
+    done
+
+  subgoal (* this one is a central argument, I didn't see this in the beginning - nice one *)
+    by (meson atLeastLessThan_iff greaterThanLessThan_iff leI less_le_trans wo_leD)
+  subgoal
+    apply safe 
+    subgoal by linarith
+    subgoal by auto
+    done
+  subgoal by blast
+  subgoal 
+        using less_trans by blast    
+  subgoal apply simp done
+  done
+
+(*
+  oops 
   supply [[put_named_ss HOL_ss]]
   apply (all \<open>(clarsimp;fail)?\<close>)
   apply clarsimp_all
@@ -367,14 +727,18 @@ lemma qs_partition_correct:
   subgoal
     by (metis greaterThanLessThan_iff strict_itrans le_neq_implies_less)
   done    
-    
+    *)
 
 definition "partition_pivot xs\<^sub>0 l h \<equiv> doN {
   ASSERT (l\<le>h \<and> h\<le>length xs\<^sub>0 \<and> h-l\<ge>4);
-  let m = l + (h-l) div 2;
-  xs\<^sub>1 \<leftarrow> move_median_to_first l (l+1) m (h-1) xs\<^sub>0;
+  hl \<leftarrow> SPECc2 ''sub'' (-) h l;
+  d \<leftarrow> SPECc2 ''div'' (div) hl 2;
+  m \<leftarrow> SPECc2 ''add'' (+) l d;
+  l' \<leftarrow> SPECc2 ''add'' (+) l 1;
+  h' \<leftarrow> SPECc2 ''sub'' (-) h 1;
+  xs\<^sub>1 \<leftarrow> move_median_to_first l l' m h' xs\<^sub>0;
   ASSERT (l<length xs\<^sub>1 \<and> length xs\<^sub>1 = length xs\<^sub>0);
-  (xs,m) \<leftarrow> qs_partition (l+1) h l xs\<^sub>1;
+  (xs,m) \<leftarrow> qs_partition l' h l xs\<^sub>1;
 
   \<comment> \<open>TODO: Use an auxiliary lemma, instead of this assertion chain! \<close>
   ASSERT (l<m \<and> m<h);
@@ -397,25 +761,79 @@ lemma slice_LT_I_aux:
     by auto
   done
   
+
+lemma (in -)
+  SPEC_timerefine_eq_arh:
+  "timerefine R (SPEC A B') = SPEC A (\<lambda>x. timerefineA R (B' x))"
+  apply(auto simp: SPEC_def)
+  unfolding timerefine_SPECT 
+  apply auto
+  unfolding timerefineF_def timerefineA_def
+  by auto
+
+lemma (in -) timerefineA_update_apply_same_cost': 
+  "timerefineA (F(n := y)) (cost n (t::enat)) = t *m y"
+  by (auto simp: costmult_def timerefineA_def cost_def zero_acost_def timerefineA_upd_aux ) 
+
+
+lemma tt2: "hi>0 \<Longrightarrow> {hi'..hi - Suc 0} = {hi'..<hi}" by auto
+
 lemma partition_pivot_correct: "\<lbrakk>(xs,xs')\<in>Id; (l,l')\<in>Id; (h,h')\<in>Id\<rbrakk> 
-  \<Longrightarrow> partition_pivot xs l h \<le> \<Down>Id (partition3_spec xs' l' h')"
+  \<Longrightarrow> partition_pivot xs l h \<le> \<Down>Id (timerefine (TId(''partition'':=qs_body_cost + move_median_to_first_cost + cost ''sub'' 2 + cost ''add'' 2 + cost ''div'' 1)) (partition3_spec xs' l' h'))"
   unfolding partition_pivot_def partition3_spec_def
-  apply (refine_vcg move_median_to_first_correct'' qs_partition_correct)
-  apply (all \<open>auto 0 3 dest: slice_eq_mset_eq_length; fail\<close>) [17]
+  apply(intro ASSERT_D3_leI)
+  apply(subst SPEC_timerefine_eq_arh)
+  unfolding SPEC_def SPECc2_def
+  apply simp
+  apply(rule gwp_specifies_I)
+  supply mmtf = move_median_to_first_correct''[unfolded SPEC_def, THEN gwp_specifies_rev_I, THEN gwp_conseq_0]
+  supply qsp = qs_partition_correct[unfolded SPEC_def, THEN gwp_specifies_rev_I, THEN gwp_conseq_0]
+  apply (refine_vcg \<open>-\<close> rules: mmtf qsp if_rule2)
+
+  apply(simp_all only: handy_if_lemma)
+
+  subgoal by auto
+  subgoal by auto
+  subgoal by auto
+  subgoal by auto
   apply clarsimp
-  subgoal for xs\<^sub>1 xs\<^sub>2 i m j
-    apply (subst slice_eq_mset_nth_outside, assumption)
-    apply (auto dest: slice_eq_mset_eq_length)
+  subgoal by auto
+  subgoal by (metis le_less_trans less_imp_diff_less linorder_not_less tt2 zero_less_numeral)
+  subgoal apply auto
+    unfolding move_median_to_first_cost_def qs_partition_cost_def
+      apply(auto simp: timerefineA_update_apply_same_cost' costmult_add_distrib costmult_cost lift_acost_cost lift_acost_propagate) 
+    apply sc_solve
+    apply safe
+    subgoal by (simp add: one_enat_def numeral_eq_enat)
+    subgoal by (simp add: one_enat_def numeral_eq_enat)
+    subgoal by (simp add: one_enat_def numeral_eq_enat)
+    subgoal by (simp add: one_enat_def numeral_eq_enat)
+    subgoal by (simp add: one_enat_def numeral_eq_enat)
+    subgoal by (simp add: one_enat_def numeral_eq_enat)
+    subgoal by (simp add: one_enat_def numeral_eq_enat)
+    subgoal by (simp add: one_enat_def numeral_eq_enat)
     done
-  subgoal apply clarsimp by (metis (full_types) Suc_leI atLeastLessThan_iff le_neq_implies_less)
-  subgoal by auto  
+  subgoal
+    apply safe
+    subgoal 
+      apply simp
+      by (metis Suc_le_eq le_add2 le_refl order.strict_trans plus_1_eq_Suc slice_eq_mset_subslice slice_eq_mset_trans)
+    subgoal by (auto dest: slice_eq_mset_eq_length intro!: slice_LT_I_aux)
+    done
   subgoal 
-    apply simp
-    by (metis Suc_le_eq le_add2 le_refl order.strict_trans plus_1_eq_Suc slice_eq_mset_subslice slice_eq_mset_trans)
-  apply (all \<open>auto; fail\<close>) [2]
-  subgoal by (auto dest: slice_eq_mset_eq_length intro!: slice_LT_I_aux)
+    by clarsimp
+  subgoal apply clarsimp by (metis (full_types) Suc_leI atLeastLessThan_iff le_neq_implies_less)
+  subgoal 
+    apply clarsimp 
+    apply (subst slice_eq_mset_nth_outside, assumption)
+      apply (auto dest: slice_eq_mset_eq_length)
+    done 
+  subgoal by auto
+  subgoal by (metis diff_is_0_eq' le_trans nat_less_le not_numeral_le_zero slice_eq_mset_eq_length)
+  subgoal by auto
   done
   
+    
 end  
   
 context sort_impl_context begin
